io/Compiler.Model2.fst
@@ -45,7 +45,7 @@ type prog_src (i:src_interface) = #fl:erased tflag -> i.pt (fl+IOActions)
 type whole_src = mst:mstate & post:(trace -> int -> trace -> Type0) & (unit -> MIO int AllActions mst (fun _ -> True) post)
 
 let link_src (#i:src_interface) (p:prog_src i) (c:ctx_src i) : whole_src =
-  (| i.mst, (fun h _ lt -> enforced_locally i.sgm h lt), (c #AllActions (inst_io_cmds i.pi) (make_dcs_eff i.pt_dcs) (p #AllActions)) |)
+  (| i.mst, (fun h _ lt -> enforced_locally i.sgm h lt), (c #AllActions (inst_io_lib i.pi) (make_dcs_eff i.pt_dcs) (p #AllActions)) |)
 
 val beh_src : whole_src ^-> trace_property #event
 let beh_src = on_domain whole_src (fun (| mst,  _, ws |) -> beh mst ws)
@@ -62,7 +62,7 @@ type prog_tgt (i:tgt_interface) = i.pt AllActions
 type whole_tgt = mst:mstate & (unit -> MIO int AllActions mst (fun _ -> True) (fun _ _ _ -> True))
 
 let link_tgt (#i:tgt_interface) (p:prog_tgt i) (c:ctx_tgt i) : whole_tgt =
-  (| i.mst, (c #AllActions (inst_io_cmds i.pi) p) |)
+  (| i.mst, (c #AllActions (inst_io_lib i.pi) p) |)
 
 val beh_tgt : whole_tgt ^-> trace_property #event
 let beh_tgt = on_domain whole_tgt (fun (| mst, wt |) -> beh mst wt)
