io/Compiler.ModelStlc.fst
@@ -82,7 +82,7 @@ type prog_src (i:src_interface) = #fl:erased tflag -> i.ct (fl+IOActions) -> uni
 type whole_src = mst:mstate & post:(trace -> int -> trace -> Type0) & (unit -> MIO int AllActions mst (fun _ -> True) post)
 
 let link_src (#i:src_interface) (p:prog_src i) (c:ctx_src i) : whole_src = 
-  (| i.mst, i.psi,  p #AllActions (c #AllActions (inst_io_cmds i.pi) (make_dcs_eff i.ct_dcs)) |)
+  (| i.mst, i.psi,  p #AllActions (c #AllActions (inst_io_lib i.pi) (make_dcs_eff i.ct_dcs)) |)
 
 val beh_src : whole_src ^-> trace_property #event
 let beh_src = on_domain whole_src (fun (| mst, _, ws |) -> beh mst ws)
@@ -100,7 +100,7 @@ type whole_tgt = mst:mstate & (unit -> MIO int AllActions mst (fun _ -> True) (f
 
 let link_tgt (#i:tgt_interface) (p:prog_tgt i) (c:ctx_tgt i) : whole_tgt =
   let (| e, h |) = c in
-  let sec_io = inst_io_cmds i.pi in
+  let sec_io = inst_io_lib i.pi in
   let c' = bt_ctx e i.ct h #AllActions #i.sgm #i.mst sec_io in
   (| i.mst , p c' |)
 
